Improve confidential and authenticated messages post-conditions; Improve request_message properties; Adapt to new FStar changes

src/lib/communication/DY.Lib.Communication.Core.Properties.fst
@@ -22,10 +22,10 @@ open DY.Lib.Communication.Core.Lemmas
 
 (*** Confidential Messages Properties ***)
 
-val conf_message_secrecy:
+val conf_message_properties:
   {|protocol_invariants|} ->
   #a:Type -> {|comm_layer_core_config a|} ->
-  tr:trace -> i:timestamp ->
+  tr:trace ->
   higher_layer_preds:comm_core_higher_layer_event_preds a ->
   receiver:principal ->
   payload:a ->
@@ -33,29 +33,30 @@ val conf_message_secrecy:
   (requires
     trace_invariant tr /\
     has_communication_layer_core_predicates higher_layer_preds /\
-    event_triggered_at tr i receiver (CommConfReceiveMsg receiver payload <: communication_core_event a)
+    event_triggered tr receiver (CommConfReceiveMsg receiver payload <: communication_core_event a)
   )
   (ensures
-    is_well_formed a (is_knowable_by (principal_label receiver) (prefix tr i)) payload /\
-    ((exists sender. higher_layer_preds.send_conf (prefix tr i) sender receiver payload) \/
-    is_well_formed a (is_publishable (prefix tr i)) payload)
+    is_well_formed a (is_knowable_by (principal_label receiver) tr) payload /\
+    ((exists sender. higher_layer_preds.send_conf tr sender receiver payload) \/
+    is_well_formed a (is_publishable tr) payload)
   )
-let conf_message_secrecy #invs #a tr i higher_layer_preds receiver payload =
+let conf_message_properties #invs #a tr higher_layer_preds receiver payload =
   let send_event sender:communication_core_event a = CommConfSendMsg sender receiver payload in
+  let i = find_event_triggered_at_timestamp tr receiver (CommConfReceiveMsg receiver payload <: communication_core_event a) in
   let tr_i = prefix tr i in
   eliminate (exists sender. event_triggered tr_i sender (send_event sender)) \/
             is_well_formed a (is_publishable tr_i) payload
   returns
-    is_well_formed a (is_knowable_by (principal_label receiver) tr_i) payload /\
-    ((exists sender. higher_layer_preds.send_conf (prefix tr i) sender receiver payload) \/
-    is_well_formed a (is_publishable (prefix tr i)) payload)
-  with _. eliminate exists sender. event_triggered tr_i sender (send_event sender)
+    is_well_formed a (is_knowable_by (principal_label receiver) tr) payload /\
+    ((exists sender. higher_layer_preds.send_conf tr sender receiver payload) \/
+    is_well_formed a (is_publishable tr) payload)
+  with _. eliminate exists sender. event_triggered (prefix tr i) sender (send_event sender)
     returns _
     with _. (
       let j = find_event_triggered_at_timestamp tr sender (send_event sender) in
       find_event_triggered_at_timestamp_later tr_i tr sender (send_event sender);
 
-      higher_layer_preds.send_conf_later (prefix tr j) tr_i sender receiver payload;
+      higher_layer_preds.send_conf_later (prefix tr j) tr sender receiver payload;
       ()
     )
   and _. ()
@@ -103,3 +104,39 @@ val sender_confauth_authentication:
     is_corrupt (prefix tr i) (long_term_key_label sender)
   )
 let sender_confauth_authentication #tag #invs #a tr i higher_layer_preds sender receiver secret = ()
+
+val confauth_message_properties:
+  {|protocol_invariants|} ->
+  #a:Type -> {|comm_layer_core_config a|} ->
+  tr:trace ->
+  higher_layer_preds:comm_core_higher_layer_event_preds a ->
+  sender:principal -> receiver:principal ->
+  payload:a ->
+  Lemma
+  (requires
+    trace_invariant tr /\
+    has_communication_layer_core_predicates higher_layer_preds /\
+    event_triggered tr receiver (CommConfAuthReceiveMsg sender receiver payload <: communication_core_event a)
+  )
+  (ensures
+    is_well_formed a (is_knowable_by (principal_label receiver) tr) payload /\
+    (higher_layer_preds.send_conf_auth tr sender receiver payload \/
+    is_corrupt tr (long_term_key_label sender))
+  )
+let confauth_message_properties #invs #a tr higher_layer_preds sender receiver payload =
+  let send_event:communication_core_event a = CommConfAuthSendMsg sender receiver payload in
+  let i = find_event_triggered_at_timestamp tr receiver (CommConfAuthReceiveMsg sender receiver payload <: communication_core_event a) in
+  let tr_i = prefix tr i in
+  eliminate event_triggered tr_i sender send_event \/ is_corrupt tr_i (long_term_key_label sender)
+  returns
+    is_well_formed a (is_knowable_by (principal_label receiver) tr) payload /\
+    (higher_layer_preds.send_conf_auth tr sender receiver payload \/
+    is_corrupt tr (long_term_key_label sender))
+  with _. (
+    let j = find_event_triggered_at_timestamp tr sender send_event in
+    find_event_triggered_at_timestamp_later tr_i tr sender send_event;
+
+    higher_layer_preds.send_conf_auth_later (prefix tr j) tr sender receiver payload;
+    ()
+  )
+  and _. ()
